Source/DafnyCore/DafnyPreludeISetAxiom.bpl
@@ -4,19 +4,19 @@ axiom (forall t: Ty :: { TISet(t) }     Tag(TISet(t))     == TagISet);
 
 function Inv0_TISet(Ty) : Ty;
 
-const unique TagISet     : TyTag;
+const unique TagISet    : TyTag;
 
 axiom (forall bx : Box, t : Ty ::
     { $IsBox(bx, TISet(t)) }
-    ( $IsBox(bx, TISet(t)) ==> $Box($Unbox(bx) : ISet Box) == bx && $Is($Unbox(bx) : ISet Box, TISet(t))));
+    ( $IsBox(bx, TISet(t)) ==> $Box($Unbox(bx) : ISet) == bx && $Is($Unbox(bx) : ISet, TISet(t))));
 
-axiom (forall v: ISet Box, t0: Ty :: { $Is(v, TISet(t0)) }
+axiom (forall v: ISet, t0: Ty :: { $Is(v, TISet(t0)) }
   $Is(v, TISet(t0)) <==>
   (forall bx: Box :: { v[bx] }
     v[bx] ==> $IsBox(bx, t0)));
 
 #if USE_HEAP
-axiom (forall v: ISet Box, t0: Ty, h: Heap :: { $IsAlloc(v, TISet(t0), h) }
+axiom (forall v: ISet, t0: Ty, h: Heap :: { $IsAlloc(v, TISet(t0), h) }
   $IsAlloc(v, TISet(t0), h) <==>
   (forall bx: Box :: { v[bx] }
     v[bx] ==> $IsAllocBox(bx, t0, h)));
@@ -25,65 +25,65 @@ axiom (forall v: ISet Box, t0: Ty, h: Heap :: { $IsAlloc(v, TISet(t0), h) }
 // -- Axiomatization of isets -------------------------------------
 // ---------------------------------------------------------------
 
-type ISet T = [T]bool;
+type ISet = [Box]bool;
 
-function ISet#Empty<T>(): Set T;
-axiom (forall<T> o: T :: { ISet#Empty()[o] } !ISet#Empty()[o]);
+function ISet#Empty(): Set;
+axiom (forall o: Box :: { ISet#Empty()[o] } !ISet#Empty()[o]);
 
 // the empty set could be of anything
-//axiom (forall<T> t: Ty :: { $Is(ISet#Empty() : [T]bool, TISet(t)) } $Is(ISet#Empty() : [T]bool, TISet(t)));
+//axiom (forall t: Ty :: { $Is(ISet#Empty() : [Box]bool, TISet(t)) } $Is(ISet#Empty() : [Box]bool, TISet(t)));
 
 
-function ISet#UnionOne<T>(ISet T, T): ISet T;
-axiom (forall<T> a: ISet T, x: T, o: T :: { ISet#UnionOne(a,x)[o] }
+function ISet#UnionOne(ISet, Box): ISet;
+axiom (forall a: ISet, x: Box, o: Box :: { ISet#UnionOne(a,x)[o] }
   ISet#UnionOne(a,x)[o] <==> o == x || a[o]);
-axiom (forall<T> a: ISet T, x: T :: { ISet#UnionOne(a, x) }
+axiom (forall a: ISet, x: Box :: { ISet#UnionOne(a, x) }
   ISet#UnionOne(a, x)[x]);
-axiom (forall<T> a: ISet T, x: T, y: T :: { ISet#UnionOne(a, x), a[y] }
+axiom (forall a: ISet, x: Box, y: Box :: { ISet#UnionOne(a, x), a[y] }
   a[y] ==> ISet#UnionOne(a, x)[y]);
 
-function ISet#Union<T>(ISet T, ISet T): ISet T;
-axiom (forall<T> a: ISet T, b: ISet T, o: T :: { ISet#Union(a,b)[o] }
+function ISet#Union(ISet, ISet): ISet;
+axiom (forall a: ISet, b: ISet, o: Box :: { ISet#Union(a,b)[o] }
   ISet#Union(a,b)[o] <==> a[o] || b[o]);
-axiom (forall<T> a, b: ISet T, y: T :: { ISet#Union(a, b), a[y] }
+axiom (forall a, b: ISet, y: Box :: { ISet#Union(a, b), a[y] }
   a[y] ==> ISet#Union(a, b)[y]);
-axiom (forall<T> a, b: Set T, y: T :: { ISet#Union(a, b), b[y] }
+axiom (forall a, b: Set, y: Box :: { ISet#Union(a, b), b[y] }
   b[y] ==> ISet#Union(a, b)[y]);
-axiom (forall<T> a, b: ISet T :: { ISet#Union(a, b) }
+axiom (forall a, b: ISet :: { ISet#Union(a, b) }
   ISet#Disjoint(a, b) ==>
     ISet#Difference(ISet#Union(a, b), a) == b &&
     ISet#Difference(ISet#Union(a, b), b) == a);
 
-function ISet#Intersection<T>(ISet T, ISet T): ISet T;
-axiom (forall<T> a: ISet T, b: ISet T, o: T :: { ISet#Intersection(a,b)[o] }
+function ISet#Intersection(ISet, ISet): ISet;
+axiom (forall a: ISet, b: ISet, o: Box :: { ISet#Intersection(a,b)[o] }
   ISet#Intersection(a,b)[o] <==> a[o] && b[o]);
 
-axiom (forall<T> a, b: ISet T :: { ISet#Union(ISet#Union(a, b), b) }
+axiom (forall a, b: ISet :: { ISet#Union(ISet#Union(a, b), b) }
   ISet#Union(ISet#Union(a, b), b) == ISet#Union(a, b));
-axiom (forall<T> a, b: Set T :: { ISet#Union(a, ISet#Union(a, b)) }
+axiom (forall a, b: Set :: { ISet#Union(a, ISet#Union(a, b)) }
   ISet#Union(a, ISet#Union(a, b)) == ISet#Union(a, b));
-axiom (forall<T> a, b: ISet T :: { ISet#Intersection(ISet#Intersection(a, b), b) }
+axiom (forall a, b: ISet :: { ISet#Intersection(ISet#Intersection(a, b), b) }
   ISet#Intersection(ISet#Intersection(a, b), b) == ISet#Intersection(a, b));
-axiom (forall<T> a, b: ISet T :: { ISet#Intersection(a, ISet#Intersection(a, b)) }
+axiom (forall a, b: ISet :: { ISet#Intersection(a, ISet#Intersection(a, b)) }
   ISet#Intersection(a, ISet#Intersection(a, b)) == ISet#Intersection(a, b));
 
 
-function ISet#Difference<T>(ISet T, ISet T): ISet T;
-axiom (forall<T> a: ISet T, b: ISet T, o: T :: { ISet#Difference(a,b)[o] }
+function ISet#Difference(ISet, ISet): ISet;
+axiom (forall a: ISet, b: ISet, o: Box :: { ISet#Difference(a,b)[o] }
   ISet#Difference(a,b)[o] <==> a[o] && !b[o]);
-axiom (forall<T> a, b: ISet T, y: T :: { ISet#Difference(a, b), b[y] }
+axiom (forall a, b: ISet, y: Box :: { ISet#Difference(a, b), b[y] }
   b[y] ==> !ISet#Difference(a, b)[y] );
 
-function ISet#Subset<T>(ISet T, ISet T): bool;
-axiom (forall<T> a: ISet T, b: ISet T :: { ISet#Subset(a,b) }
-  ISet#Subset(a,b) <==> (forall o: T :: {a[o]} {b[o]} a[o] ==> b[o]));
+function ISet#Subset(ISet, ISet): bool;
+axiom (forall a: ISet, b: ISet :: { ISet#Subset(a,b) }
+  ISet#Subset(a,b) <==> (forall o: Box :: {a[o]} {b[o]} a[o] ==> b[o]));
 
-function ISet#Equal<T>(ISet T, ISet T): bool;
-axiom (forall<T> a: ISet T, b: ISet T :: { ISet#Equal(a,b) }
-  ISet#Equal(a,b) <==> (forall o: T :: {a[o]} {b[o]} a[o] <==> b[o]));
-axiom (forall<T> a: ISet T, b: ISet T :: { ISet#Equal(a,b) }  // extensionality axiom for sets
+function ISet#Equal(ISet, ISet): bool;
+axiom (forall a: ISet, b: ISet :: { ISet#Equal(a,b) }
+  ISet#Equal(a,b) <==> (forall o: Box :: {a[o]} {b[o]} a[o] <==> b[o]));
+axiom (forall a: ISet, b: ISet :: { ISet#Equal(a,b) }  // extensionality axiom for sets
   ISet#Equal(a,b) ==> a == b);
 
-function ISet#Disjoint<T>(ISet T, ISet T): bool;
-axiom (forall<T> a: ISet T, b: ISet T :: { ISet#Disjoint(a,b) }
-  ISet#Disjoint(a,b) <==> (forall o: T :: {a[o]} {b[o]} !a[o] || !b[o]));
+function ISet#Disjoint(ISet, ISet): bool;
+axiom (forall a: ISet, b: ISet :: { ISet#Disjoint(a,b) }
+  ISet#Disjoint(a,b) <==> (forall o: Box :: {a[o]} {b[o]} !a[o] || !b[o]));
