Source/DafnyCore/DafnyPreludeMapAxiom.bpl
@@ -10,9 +10,9 @@ const unique TagMap      : TyTag;
 
 axiom (forall bx : Box, s : Ty, t : Ty ::
     { $IsBox(bx, TMap(s, t)) }
-    ( $IsBox(bx, TMap(s, t)) ==> $Box($Unbox(bx) : Map Box Box) == bx && $Is($Unbox(bx) : Map Box Box, TMap(s, t))));
+    ( $IsBox(bx, TMap(s, t)) ==> $Box($Unbox(bx) : Map) == bx && $Is($Unbox(bx) : Map, TMap(s, t))));
 
-axiom (forall v: Map Box Box, t0: Ty, t1: Ty ::
+axiom (forall v: Map, t0: Ty, t1: Ty ::
   { $Is(v, TMap(t0, t1)) }
   $Is(v, TMap(t0, t1))
      <==> (forall bx: Box ::
@@ -21,7 +21,7 @@ axiom (forall v: Map Box Box, t0: Ty, t1: Ty ::
         $IsBox(Map#Elements(v)[bx], t1) &&
         $IsBox(bx, t0)));
             
-axiom (forall v: Map Box Box, t0: Ty, t1: Ty ::
+axiom (forall v: Map, t0: Ty, t1: Ty ::
   { $Is(v, TMap(t0, t1)) }
   $Is(v, TMap(t0, t1)) ==>
     $Is(Map#Domain(v), TSet(t0)) &&
@@ -29,7 +29,7 @@ axiom (forall v: Map Box Box, t0: Ty, t1: Ty ::
     $Is(Map#Items(v), TSet(Tclass._System.Tuple2(t0, t1))));
 
 #if USE_HEAP
-axiom (forall v: Map Box Box, t0: Ty, t1: Ty, h: Heap ::
+axiom (forall v: Map, t0: Ty, t1: Ty, h: Heap ::
   { $IsAlloc(v, TMap(t0, t1), h) }
   $IsAlloc(v, TMap(t0, t1), h)
      <==> (forall bx: Box ::
@@ -42,39 +42,39 @@ axiom (forall v: Map Box Box, t0: Ty, t1: Ty, h: Heap ::
 // -- Axiomatization of Maps -------------------------------------
 // ---------------------------------------------------------------
 
-type Map U V;
+type Map;
 
 // A Map is defined by three functions, Map#Domain, Map#Elements, and #Map#Card.
 
-function Map#Domain<U,V>(Map U V) : Set U;
+function Map#Domain(Map) : Set;
 
-function Map#Elements<U,V>(Map U V) : [U]V;
+function Map#Elements(Map) : [Box]Box;
 
-function Map#Card<U,V>(Map U V) : int;
+function Map#Card(Map) : int;
 
-axiom (forall<U,V> m: Map U V :: { Map#Card(m) } 0 <= Map#Card(m));
+axiom (forall m: Map :: { Map#Card(m) } 0 <= Map#Card(m));
 
-axiom (forall<U, V> m: Map U V ::
+axiom (forall m: Map ::
   { Map#Card(m) }
   Map#Card(m) == 0 <==> m == Map#Empty());
 
-axiom (forall<U, V> m: Map U V ::
+axiom (forall m: Map ::
   { Map#Domain(m) }
-  m == Map#Empty() || (exists k: U :: Map#Domain(m)[k]));
-axiom (forall<U, V> m: Map U V ::
+  m == Map#Empty() || (exists k: Box :: Map#Domain(m)[k]));
+axiom (forall m: Map ::
   { Map#Values(m) }
-  m == Map#Empty() || (exists v: V :: Map#Values(m)[v]));
-axiom (forall<U, V> m: Map U V ::
+  m == Map#Empty() || (exists v: Box :: Map#Values(m)[v]));
+axiom (forall m: Map ::
   { Map#Items(m) }
   m == Map#Empty() || (exists k, v: Box :: Map#Items(m)[$Box(#_System._tuple#2._#Make2(k, v))]));
 
-axiom (forall<U, V> m: Map U V ::
+axiom (forall m: Map ::
   { Set#Card(Map#Domain(m)) } { Map#Card(m) }
   Set#Card(Map#Domain(m)) == Map#Card(m));
-axiom (forall<U, V> m: Map U V ::
+axiom (forall m: Map ::
   { Set#Card(Map#Values(m)) } { Map#Card(m) }
   Set#Card(Map#Values(m)) <= Map#Card(m));
-axiom (forall<U, V> m: Map U V ::
+axiom (forall m: Map ::
   { Set#Card(Map#Items(m)) } { Map#Card(m) }
   Set#Card(Map#Items(m)) == Map#Card(m));
 
@@ -83,42 +83,42 @@ axiom (forall<U, V> m: Map U V ::
 // square brackets) and Map#Card, so we need to define what these mean for the Set
 // returned by Map#Values.
 
-function Map#Values<U,V>(Map U V) : Set V;
+function Map#Values(Map) : Set;
 
-axiom (forall<U,V> m: Map U V, v: V :: { Map#Values(m)[v] }
+axiom (forall m: Map, v: Box :: { Map#Values(m)[v] }
   Map#Values(m)[v] ==
-	(exists u: U :: { Map#Domain(m)[u] } { Map#Elements(m)[u] }
+	(exists u: Box :: { Map#Domain(m)[u] } { Map#Elements(m)[u] }
 	  Map#Domain(m)[u] &&
     v == Map#Elements(m)[u]));
 
 // The set of Items--that is, (key,value) pairs--of a Map can be obtained by the
 // function Map#Items.  Again, we need to define membership of Set#Card for this
-// set.  Everywhere else in this axiomatization, Map is parameterized by types U V,
+// set.  Everywhere else in this axiomatization, Map is parameterized by types Box V,
 // even though Dafny only ever instantiates U V with Box Box.  This makes the
 // axiomatization more generic.  Function Map#Items, however, returns a set of
 // pairs, and the axiomatization of pairs is Dafny specific.  Therefore, the
 // definition of Map#Items here is to be considered Dafny specific.  Also, note
 // that it relies on the two destructors for 2-tuples.
 
-function Map#Items<U,V>(Map U V) : Set Box;
+function Map#Items(Map) : Set;
 
-axiom (forall m: Map Box Box, item: Box :: { Map#Items(m)[item] }
+axiom (forall m: Map, item: Box :: { Map#Items(m)[item] }
   Map#Items(m)[item] <==>
     Map#Domain(m)[_System.Tuple2._0($Unbox(item))] &&
     Map#Elements(m)[_System.Tuple2._0($Unbox(item))] == _System.Tuple2._1($Unbox(item)));
 
 // Here are the operations that produce Map values.
 
-function Map#Empty<U, V>(): Map U V;
-axiom (forall<U, V> u: U ::
-        { Map#Domain(Map#Empty(): Map U V)[u] }
-        !Map#Domain(Map#Empty(): Map U V)[u]);
+function Map#Empty(): Map;
+axiom (forall u: Box ::
+        { Map#Domain(Map#Empty(): Map)[u] }
+        !Map#Domain(Map#Empty(): Map)[u]);
 
-function Map#Glue<U, V>([U]bool, [U]V, Ty): Map U V;
-axiom (forall<U, V> a: [U]bool, b: [U]V, t: Ty ::
+function Map#Glue([Box]bool, [Box]Box, Ty): Map;
+axiom (forall a: [Box]bool, b: [Box]Box, t: Ty ::
   { Map#Domain(Map#Glue(a, b, t)) }
   Map#Domain(Map#Glue(a, b, t)) == a);
-axiom (forall<U, V> a: [U]bool, b: [U]V, t: Ty ::
+axiom (forall a: [Box]bool, b: [Box]Box, t: Ty ::
   { Map#Elements(Map#Glue(a, b, t)) }
   Map#Elements(Map#Glue(a, b, t)) == b);
 axiom (forall a: [Box]bool, b: [Box]Box, t0, t1: Ty ::
@@ -130,54 +130,54 @@ axiom (forall a: [Box]bool, b: [Box]Box, t0, t1: Ty ::
 
 
 //Build is used in displays, and for map updates
-function Map#Build<U, V>(Map U V, U, V): Map U V;
-/*axiom (forall<U, V> m: Map U V, u: U, v: V ::
+function Map#Build(Map, Box, Box): Map;
+/*axiom (forall m: Map, u: Box, v: Box ::
   { Map#Domain(Map#Build(m, u, v))[u] } { Map#Elements(Map#Build(m, u, v))[u] }
   Map#Domain(Map#Build(m, u, v))[u] && Map#Elements(Map#Build(m, u, v))[u] == v);*/
 
-axiom (forall<U, V> m: Map U V, u: U, u': U, v: V ::
+axiom (forall m: Map, u: Box, u': Box, v: Box ::
   { Map#Domain(Map#Build(m, u, v))[u'] } { Map#Elements(Map#Build(m, u, v))[u'] }
   (u' == u ==> Map#Domain(Map#Build(m, u, v))[u'] &&
                Map#Elements(Map#Build(m, u, v))[u'] == v) &&
   (u' != u ==> Map#Domain(Map#Build(m, u, v))[u'] == Map#Domain(m)[u'] &&
                Map#Elements(Map#Build(m, u, v))[u'] == Map#Elements(m)[u']));
-axiom (forall<U, V> m: Map U V, u: U, v: V :: { Map#Card(Map#Build(m, u, v)) }
+axiom (forall m: Map, u: Box, v: Box :: { Map#Card(Map#Build(m, u, v)) }
   Map#Domain(m)[u] ==> Map#Card(Map#Build(m, u, v)) == Map#Card(m));
-axiom (forall<U, V> m: Map U V, u: U, v: V :: { Map#Card(Map#Build(m, u, v)) }
+axiom (forall m: Map, u: Box, v: Box :: { Map#Card(Map#Build(m, u, v)) }
   !Map#Domain(m)[u] ==> Map#Card(Map#Build(m, u, v)) == Map#Card(m) + 1);
 
 // Map operations
-function Map#Merge<U, V>(Map U V, Map U V): Map U V;
-axiom (forall<U, V> m: Map U V, n: Map U V ::
+function Map#Merge(Map, Map): Map;
+axiom (forall m: Map, n: Map ::
   { Map#Domain(Map#Merge(m, n)) }
   Map#Domain(Map#Merge(m, n)) == Set#Union(Map#Domain(m), Map#Domain(n)));
-axiom (forall<U, V> m: Map U V, n: Map U V, u: U ::
+axiom (forall m: Map, n: Map, u: Box ::
   { Map#Elements(Map#Merge(m, n))[u] }
   Map#Domain(Map#Merge(m, n))[u] ==>
     (!Map#Domain(n)[u] ==> Map#Elements(Map#Merge(m, n))[u] == Map#Elements(m)[u]) &&
     (Map#Domain(n)[u] ==> Map#Elements(Map#Merge(m, n))[u] == Map#Elements(n)[u]));
 
-function Map#Subtract<U, V>(Map U V, Set U): Map U V;
-axiom (forall<U, V> m: Map U V, s: Set U ::
+function Map#Subtract(Map, Set): Map;
+axiom (forall m: Map, s: Set ::
   { Map#Domain(Map#Subtract(m, s)) }
   Map#Domain(Map#Subtract(m, s)) == Set#Difference(Map#Domain(m), s));
-axiom (forall<U, V> m: Map U V, s: Set U, u: U ::
+axiom (forall m: Map, s: Set, u: Box ::
   { Map#Elements(Map#Subtract(m, s))[u] }
   Map#Domain(Map#Subtract(m, s))[u] ==>
     Map#Elements(Map#Subtract(m, s))[u] == Map#Elements(m)[u]);
 
 //equality for maps
-function Map#Equal<U, V>(Map U V, Map U V): bool;
-axiom (forall<U, V> m: Map U V, m': Map U V::
+function Map#Equal(Map, Map): bool;
+axiom (forall m: Map, m': Map::
   { Map#Equal(m, m') }
-    Map#Equal(m, m') <==> (forall u : U :: Map#Domain(m)[u] == Map#Domain(m')[u]) &&
-                          (forall u : U :: Map#Domain(m)[u] ==> Map#Elements(m)[u] == Map#Elements(m')[u]));
+    Map#Equal(m, m') <==> (forall u : Box :: Map#Domain(m)[u] == Map#Domain(m')[u]) &&
+                          (forall u : Box :: Map#Domain(m)[u] ==> Map#Elements(m)[u] == Map#Elements(m')[u]));
 // extensionality
-axiom (forall<U, V> m: Map U V, m': Map U V::
+axiom (forall m: Map, m': Map::
   { Map#Equal(m, m') }
     Map#Equal(m, m') ==> m == m');
 
-function Map#Disjoint<U, V>(Map U V, Map U V): bool;
-axiom (forall<U, V> m: Map U V, m': Map U V ::
+function Map#Disjoint(Map, Map): bool;
+axiom (forall m: Map, m': Map ::
   { Map#Disjoint(m, m') }
-    Map#Disjoint(m, m') <==> (forall o: U :: {Map#Domain(m)[o]} {Map#Domain(m')[o]} !Map#Domain(m)[o] || !Map#Domain(m')[o]));
+    Map#Disjoint(m, m') <==> (forall o: Box :: {Map#Domain(m)[o]} {Map#Domain(m')[o]} !Map#Domain(m)[o] || !Map#Domain(m')[o]));
