Source/DafnyCore/DafnyPreludeMultiSetAxiom.bpl
@@ -8,17 +8,17 @@ const unique TagMultiSet : TyTag;
 
 axiom (forall bx : Box, t : Ty ::
     { $IsBox(bx, TMultiSet(t)) }
-    ( $IsBox(bx, TMultiSet(t)) ==> $Box($Unbox(bx) : MultiSet Box) == bx && $Is($Unbox(bx) : MultiSet Box, TMultiSet(t))));
+    ( $IsBox(bx, TMultiSet(t)) ==> $Box($Unbox(bx) : MultiSet) == bx && $Is($Unbox(bx) : MultiSet, TMultiSet(t))));
 
-axiom (forall v: MultiSet Box, t0: Ty :: { $Is(v, TMultiSet(t0)) }
+axiom (forall v: MultiSet, t0: Ty :: { $Is(v, TMultiSet(t0)) }
   $Is(v, TMultiSet(t0)) <==>
   (forall bx: Box :: { v[bx] }
     0 < v[bx] ==> $IsBox(bx, t0)));
-axiom (forall v: MultiSet Box, t0: Ty :: { $Is(v, TMultiSet(t0)) }
+axiom (forall v: MultiSet, t0: Ty :: { $Is(v, TMultiSet(t0)) }
   $Is(v, TMultiSet(t0)) ==> $IsGoodMultiSet(v));
 
 #if USE_HEAP
-axiom (forall v: MultiSet Box, t0: Ty, h: Heap :: { $IsAlloc(v, TMultiSet(t0), h) }
+axiom (forall v: MultiSet, t0: Ty, h: Heap :: { $IsAlloc(v, TMultiSet(t0), h) }
   $IsAlloc(v, TMultiSet(t0), h) <==>
   (forall bx: Box :: { v[bx] }
     0 < v[bx] ==> $IsAllocBox(bx, t0, h)));
@@ -37,71 +37,71 @@ function Math#clip(a: int): int;
 axiom (forall a: int :: { Math#clip(a) } 0 <= a ==> Math#clip(a) == a);
 axiom (forall a: int :: { Math#clip(a) } a < 0  ==> Math#clip(a) == 0);
 
-type MultiSet T = [T]int;
+type MultiSet = [Box]int;
 
-function $IsGoodMultiSet<T>(ms: MultiSet T): bool;
+function $IsGoodMultiSet(ms: MultiSet): bool;
 // ints are non-negative, used after havocing, and for conversion from sequences to multisets.
-axiom (forall<T> ms: MultiSet T :: { $IsGoodMultiSet(ms) }
+axiom (forall ms: MultiSet :: { $IsGoodMultiSet(ms) }
   $IsGoodMultiSet(ms) <==>
-  (forall bx: T :: { ms[bx] } 0 <= ms[bx] && ms[bx] <= MultiSet#Card(ms)));
+  (forall bx: Box :: { ms[bx] } 0 <= ms[bx] && ms[bx] <= MultiSet#Card(ms)));
 
-function MultiSet#Card<T>(MultiSet T): int;
-axiom (forall<T> s: MultiSet T :: { MultiSet#Card(s) } 0 <= MultiSet#Card(s));
-axiom (forall<T> s: MultiSet T, x: T, n: int :: { MultiSet#Card(s[x := n]) }
+function MultiSet#Card(MultiSet): int;
+axiom (forall s: MultiSet :: { MultiSet#Card(s) } 0 <= MultiSet#Card(s));
+axiom (forall s: MultiSet, x: Box, n: int :: { MultiSet#Card(s[x := n]) }
   0 <= n ==> MultiSet#Card(s[x := n]) == MultiSet#Card(s) - s[x] + n);
 
-function MultiSet#Empty<T>(): MultiSet T;
-axiom (forall<T> o: T :: { MultiSet#Empty()[o] } MultiSet#Empty()[o] == 0);
-axiom (forall<T> s: MultiSet T :: { MultiSet#Card(s) }
+function MultiSet#Empty(): MultiSet;
+axiom (forall o: Box :: { MultiSet#Empty()[o] } MultiSet#Empty()[o] == 0);
+axiom (forall s: MultiSet :: { MultiSet#Card(s) }
   (MultiSet#Card(s) == 0 <==> s == MultiSet#Empty()) &&
-  (MultiSet#Card(s) != 0 ==> (exists x: T :: 0 < s[x])));
+  (MultiSet#Card(s) != 0 ==> (exists x: Box :: 0 < s[x])));
 
-function MultiSet#Singleton<T>(T): MultiSet T;
-axiom (forall<T> r: T, o: T :: { MultiSet#Singleton(r)[o] } (MultiSet#Singleton(r)[o] == 1 <==> r == o) &&
+function MultiSet#Singleton(Box): MultiSet;
+axiom (forall r: Box, o: Box :: { MultiSet#Singleton(r)[o] } (MultiSet#Singleton(r)[o] == 1 <==> r == o) &&
                                                             (MultiSet#Singleton(r)[o] == 0 <==> r != o));
-axiom (forall<T> r: T :: { MultiSet#Singleton(r) } MultiSet#Singleton(r) == MultiSet#UnionOne(MultiSet#Empty(), r));
+axiom (forall r: Box :: { MultiSet#Singleton(r) } MultiSet#Singleton(r) == MultiSet#UnionOne(MultiSet#Empty(), r));
 
-function MultiSet#UnionOne<T>(MultiSet T, T): MultiSet T;
+function MultiSet#UnionOne(MultiSet, Box): MultiSet;
 // pure containment axiom (in the original multiset or is the added element)
-axiom (forall<T> a: MultiSet T, x: T, o: T :: { MultiSet#UnionOne(a,x)[o] }
+axiom (forall a: MultiSet, x: Box, o: Box :: { MultiSet#UnionOne(a,x)[o] }
   0 < MultiSet#UnionOne(a,x)[o] <==> o == x || 0 < a[o]);
 // union-ing increases count by one
-axiom (forall<T> a: MultiSet T, x: T :: { MultiSet#UnionOne(a, x) }
+axiom (forall a: MultiSet, x: Box :: { MultiSet#UnionOne(a, x) }
   MultiSet#UnionOne(a, x)[x] == a[x] + 1);
 // non-decreasing
-axiom (forall<T> a: MultiSet T, x: T, y: T :: { MultiSet#UnionOne(a, x), a[y] }
+axiom (forall a: MultiSet, x: Box, y: Box :: { MultiSet#UnionOne(a, x), a[y] }
   0 < a[y] ==> 0 < MultiSet#UnionOne(a, x)[y]);
 // other elements unchanged
-axiom (forall<T> a: MultiSet T, x: T, y: T :: { MultiSet#UnionOne(a, x), a[y] }
+axiom (forall a: MultiSet, x: Box, y: Box :: { MultiSet#UnionOne(a, x), a[y] }
   x != y ==> a[y] == MultiSet#UnionOne(a, x)[y]);
-axiom (forall<T> a: MultiSet T, x: T :: { MultiSet#Card(MultiSet#UnionOne(a, x)) }
+axiom (forall a: MultiSet, x: Box :: { MultiSet#Card(MultiSet#UnionOne(a, x)) }
   MultiSet#Card(MultiSet#UnionOne(a, x)) == MultiSet#Card(a) + 1);
 
 
-function MultiSet#Union<T>(MultiSet T, MultiSet T): MultiSet T;
+function MultiSet#Union(MultiSet, MultiSet): MultiSet;
 // union-ing is the sum of the contents
-axiom (forall<T> a: MultiSet T, b: MultiSet T, o: T :: { MultiSet#Union(a,b)[o] }
+axiom (forall a: MultiSet, b: MultiSet, o: Box :: { MultiSet#Union(a,b)[o] }
   MultiSet#Union(a,b)[o] == a[o] + b[o]);
-axiom (forall<T> a: MultiSet T, b: MultiSet T :: { MultiSet#Card(MultiSet#Union(a,b)) }
+axiom (forall a: MultiSet, b: MultiSet :: { MultiSet#Card(MultiSet#Union(a,b)) }
   MultiSet#Card(MultiSet#Union(a,b)) == MultiSet#Card(a) + MultiSet#Card(b));
 
-function MultiSet#Intersection<T>(MultiSet T, MultiSet T): MultiSet T;
-axiom (forall<T> a: MultiSet T, b: MultiSet T, o: T :: { MultiSet#Intersection(a,b)[o] }
+function MultiSet#Intersection(MultiSet, MultiSet): MultiSet;
+axiom (forall a: MultiSet, b: MultiSet, o: Box :: { MultiSet#Intersection(a,b)[o] }
   MultiSet#Intersection(a,b)[o] == Math#min(a[o],  b[o]));
 
 // left and right pseudo-idempotence
-axiom (forall<T> a, b: MultiSet T :: { MultiSet#Intersection(MultiSet#Intersection(a, b), b) }
+axiom (forall a, b: MultiSet :: { MultiSet#Intersection(MultiSet#Intersection(a, b), b) }
   MultiSet#Intersection(MultiSet#Intersection(a, b), b) == MultiSet#Intersection(a, b));
-axiom (forall<T> a, b: MultiSet T :: { MultiSet#Intersection(a, MultiSet#Intersection(a, b)) }
+axiom (forall a, b: MultiSet :: { MultiSet#Intersection(a, MultiSet#Intersection(a, b)) }
   MultiSet#Intersection(a, MultiSet#Intersection(a, b)) == MultiSet#Intersection(a, b));
 
 // multiset difference, a - b. clip() makes it positive.
-function MultiSet#Difference<T>(MultiSet T, MultiSet T): MultiSet T;
-axiom (forall<T> a: MultiSet T, b: MultiSet T, o: T :: { MultiSet#Difference(a,b)[o] }
+function MultiSet#Difference(MultiSet, MultiSet): MultiSet;
+axiom (forall a: MultiSet, b: MultiSet, o: Box :: { MultiSet#Difference(a,b)[o] }
   MultiSet#Difference(a,b)[o] == Math#clip(a[o] - b[o]));
-axiom (forall<T> a, b: MultiSet T, y: T :: { MultiSet#Difference(a, b), b[y], a[y] }
+axiom (forall a, b: MultiSet, y: Box :: { MultiSet#Difference(a, b), b[y], a[y] }
   a[y] <= b[y] ==> MultiSet#Difference(a, b)[y] == 0 );
-axiom (forall<T> a, b: MultiSet T ::
+axiom (forall a, b: MultiSet ::
   { MultiSet#Card(MultiSet#Difference(a, b)) }
   MultiSet#Card(MultiSet#Difference(a, b)) + MultiSet#Card(MultiSet#Difference(b, a))
   + 2 * MultiSet#Card(MultiSet#Intersection(a, b))
@@ -109,32 +109,32 @@ axiom (forall<T> a, b: MultiSet T ::
   MultiSet#Card(MultiSet#Difference(a, b)) == MultiSet#Card(a) - MultiSet#Card(MultiSet#Intersection(a, b)));
 
 // multiset subset means a must have at most as many of each element as b
-function MultiSet#Subset<T>(MultiSet T, MultiSet T): bool;
-axiom (forall<T> a: MultiSet T, b: MultiSet T :: { MultiSet#Subset(a,b) }
-  MultiSet#Subset(a,b) <==> (forall o: T :: {a[o]} {b[o]} a[o] <= b[o]));
+function MultiSet#Subset(MultiSet, MultiSet): bool;
+axiom (forall a: MultiSet, b: MultiSet :: { MultiSet#Subset(a,b) }
+  MultiSet#Subset(a,b) <==> (forall o: Box :: {a[o]} {b[o]} a[o] <= b[o]));
 
-function MultiSet#Equal<T>(MultiSet T, MultiSet T): bool;
-axiom (forall<T> a: MultiSet T, b: MultiSet T :: { MultiSet#Equal(a,b) }
-  MultiSet#Equal(a,b) <==> (forall o: T :: {a[o]} {b[o]} a[o] == b[o]));
+function MultiSet#Equal(MultiSet, MultiSet): bool;
+axiom (forall a: MultiSet, b: MultiSet :: { MultiSet#Equal(a,b) }
+  MultiSet#Equal(a,b) <==> (forall o: Box :: {a[o]} {b[o]} a[o] == b[o]));
 // extensionality axiom for multisets
-axiom (forall<T> a: MultiSet T, b: MultiSet T :: { MultiSet#Equal(a,b) }
+axiom (forall a: MultiSet, b: MultiSet :: { MultiSet#Equal(a,b) }
   MultiSet#Equal(a,b) ==> a == b);
 
-function MultiSet#Disjoint<T>(MultiSet T, MultiSet T): bool;
-axiom (forall<T> a: MultiSet T, b: MultiSet T :: { MultiSet#Disjoint(a,b) }
-  MultiSet#Disjoint(a,b) <==> (forall o: T :: {a[o]} {b[o]} a[o] == 0 || b[o] == 0));
+function MultiSet#Disjoint(MultiSet, MultiSet): bool;
+axiom (forall a: MultiSet, b: MultiSet :: { MultiSet#Disjoint(a,b) }
+  MultiSet#Disjoint(a,b) <==> (forall o: Box :: {a[o]} {b[o]} a[o] == 0 || b[o] == 0));
 
 // conversion to a multiset. each element in the original set has duplicity 1.
-function MultiSet#FromSet<T>(Set T): MultiSet T;
-axiom (forall<T> s: Set T, a: T :: { MultiSet#FromSet(s)[a] }
+function MultiSet#FromSet(Set): MultiSet;
+axiom (forall s: Set, a: Box :: { MultiSet#FromSet(s)[a] }
   (MultiSet#FromSet(s)[a] == 0 <==> !s[a]) &&
   (MultiSet#FromSet(s)[a] == 1 <==> s[a]));
-axiom (forall<T> s: Set T :: { MultiSet#Card(MultiSet#FromSet(s)) }
+axiom (forall s: Set :: { MultiSet#Card(MultiSet#FromSet(s)) }
   MultiSet#Card(MultiSet#FromSet(s)) == Set#Card(s));
 
 // conversion to a multiset, from a sequence.
-function MultiSet#FromSeq(Seq): MultiSet Box uses {
-  axiom MultiSet#FromSeq(Seq#Empty(): Seq) == MultiSet#Empty(): MultiSet Box;
+function MultiSet#FromSeq(Seq): MultiSet uses {
+  axiom MultiSet#FromSeq(Seq#Empty(): Seq) == MultiSet#Empty(): MultiSet;
 }
 
 // conversion produces a good map.
